Sources.lean
@@ -116,6 +116,10 @@ import Sources.Doi_10_1145_321662_321665.Source
 import Sources.Doi_10_1145_321662_321665.Subresultants
 import Sources.Doi_10_1145_800204_806314.Source
 import Sources.Doi_10_1145_800204_806314.HorowitzMethod
+
+import Sources.Doi_10_1007_978_3_031_57262_3_10.Source
+import Sources.Doi_10_1007_978_3_031_57262_3_10.Section21
+import Sources.Doi_10_1007_978_3_031_57262_3_10.Theory
 import Sources.Doi_10_1007_978_3_7091_7551_4_9.Source
 import Sources.Doi_10_1007_978_3_7091_7551_4_9.SubresultantPRS
 import Sources.Doi_10_1006_jsco_1995_1043.Source
